src/AsyncFSRecover.v
@@ -1,0 +1,594 @@
+Require Import Log.
+Require Import BFile.
+Require Import Word.
+Require Import Omega.
+Require Import Prog.
+Require Import Bool.
+Require Import Pred PredCrash.
+Require Import DirName.
+Require Import Hoare.
+Require Import GenSepN.
+Require Import ListPred.
+Require Import SepAuto.
+Require Import Idempotent.
+Require Import Inode.
+Require Import List ListUtils.
+Require Import Balloc.
+Require Import Bytes.
+Require Import DirTree.
+Require Import Rec.
+Require Import Arith.
+Require Import Array.
+Require Import FSLayout.
+Require Import Errno.
+Require Import AsyncDisk.
+Require Import GroupLog.
+Require Import DiskLog.
+Require Import SuperBlock.
+Require Import DiskSet.
+Require Import AsyncFS.
+
+Set Implicit Arguments.
+Import ListNotations.
+
+
+Module AFS_RECOVER.
+
+  Import AFS.
+  Import DirTree.
+  Import DirTreeDef.
+
+  Parameter cachesize : nat.
+  Axiom cachesize_ok : cachesize <> 0.
+  Hint Resolve cachesize_ok.
+
+  Notation MSLL := BFILE.MSLL.
+  Notation MSAlloc := BFILE.MSAlloc.
+
+
+  Theorem file_getattr_recover_ok : forall pr fsxp inum mscs,
+  {X<< ds sm pathname Fm Ftop tree f ilist frees,
+  PERM:pr     
+  PRE:bm, hm,
+         LOG.rep (FSXPLog fsxp) (SB.rep fsxp) (LOG.NoTxn ds) (MSLL mscs) sm bm hm *
+         [[[ ds!! ::: (Fm * DirTreeRep.rep fsxp Ftop tree ilist frees mscs sm) ]]] *
+         [[ find_subtree pathname tree = Some (TreeFile inum f) ]]
+  POST:bm', hm', RET:^(mscs',r)
+         LOG.rep (FSXPLog fsxp) (SB.rep fsxp) (LOG.NoTxn ds) (MSLL mscs') sm bm' hm' *
+         [[ r = DFAttr f ]]
+  REC:bm'', hm', RET:r exists mscs fsxp,
+         exists d sm' n, LOG.rep (FSXPLog fsxp) (SB.rep fsxp) (LOG.NoTxn (d, nil)) (MSLL mscs) sm' bm'' hm' *
+         [[ n <= length (snd ds) ]] *
+         [[[ d ::: crash_xform (diskIs (list2nmem (nthd n ds))) ]]]
+  >>X} file_get_attr fsxp inum mscs >> recover cachesize.
+  Proof.
+    unfold forall_helper.
+    recover_ro_ok.
+    destruct v.
+    cancel.
+    eauto.
+    step.
+
+    norm'l. unfold stars; simpl.
+    cancel.
+    eassign_idempred.
+
+    simpl_idempred_l.
+    xform_norml;
+      rewrite SB.crash_xform_rep;
+      (rewrite LOG.notxn_after_crash_diskIs || rewrite LOG.rollbacktxn_after_crash_diskIs);
+      try eassumption.
+    cancel.
+
+    safestep; subst. 2: eauto.
+    simpl_idempred_r.
+    eauto.
+    simpl_idempred_r.
+    rewrite <- LOG.before_crash_idempred.
+    cancel. auto.
+
+    cancel.
+    safestep; subst. 2:eauto.
+    simpl_idempred_r.
+    eauto.
+    simpl_idempred_r.
+    rewrite <- LOG.before_crash_idempred.
+    cancel. auto.
+  Qed.
+
+
+  Theorem read_fblock_recover_ok : forall fsxp inum off mscs,
+    {X<< ds sm Fm Ftop tree pathname f Fd vs ilist frees,
+    PRE:hm LOG.rep (FSXPLog fsxp) (SB.rep fsxp) (LOG.NoTxn ds) (MSLL mscs) sm hm *
+           [[[ ds!! ::: (Fm * DirTreeRep.rep fsxp Ftop tree ilist frees mscs sm)]]] *
+           [[ find_subtree pathname tree = Some (TreeFile inum f) ]] *
+           [[[ (DFData f) ::: (Fd * off |-> vs) ]]]
+    POST:hm' RET:^(mscs', r)
+           LOG.rep (FSXPLog fsxp) (SB.rep  fsxp) (LOG.NoTxn ds) (MSLL mscs') sm hm' *
+           [[ r = fst vs ]]
+    REC:vm',hm' RET:r exists mscs fsxp,
+         exists d sm' n, LOG.rep (FSXPLog fsxp) (SB.rep fsxp) (LOG.NoTxn (d, nil)) (MSLL mscs) sm' hm' *
+         [[ n <= length (snd ds) ]] *
+         [[[ d ::: crash_xform (diskIs (list2nmem (nthd n ds))) ]]]
+    >>X} read_fblock fsxp inum off mscs >> recover cachesize.
+  Proof.
+    unfold forall_helper.
+    recover_ro_ok.
+    destruct v.
+    cancel.
+    eauto.
+    eauto.
+    step.
+
+    eassign_idempred.
+
+    simpl_idempred_l.
+    xform_norml;
+      rewrite SB.crash_xform_rep;
+      (rewrite LOG.notxn_after_crash_diskIs || rewrite LOG.rollbacktxn_after_crash_diskIs);
+      try eassumption.
+    cancel.
+    safestep; subst. 2: eauto.
+    simpl_idempred_r.
+    eassumption.
+    simpl_idempred_r.
+    rewrite <- LOG.before_crash_idempred.
+
+    cancel. auto.
+
+    cancel.
+    safestep; subst. 2:eassumption.
+    simpl_idempred_r.
+    eauto.
+    simpl_idempred_r.
+    rewrite <- LOG.before_crash_idempred.
+    cancel. auto.
+  Qed.
+
+
+  Lemma instantiate_crash : forall idemcrash (F_ : rawpred) (hm_crash : hashmap),
+    (fun hm => F_ * idemcrash hm) hm_crash =p=> F_ * idemcrash hm_crash.
+  Proof.
+    reflexivity.
+  Qed.
+
+
+  Theorem file_truncate_recover_ok : forall fsxp inum sz mscs,
+    {<< ds sm Fm Ftop tree pathname f ilist frees,
+    PRE:hm
+      LOG.rep (FSXPLog fsxp) (SB.rep fsxp) (LOG.NoTxn ds) (MSLL mscs) sm hm *
+      [[[ ds!! ::: (Fm * DirTreeRep.rep fsxp Ftop tree ilist frees mscs sm)]]] *
+      [[ find_subtree pathname tree = Some (TreeFile inum f) ]]
+    POST:hm' RET:^(mscs', r)
+      [[ isError r ]] * LOG.rep (FSXPLog fsxp) (SB.rep fsxp) (LOG.NoTxn ds) (MSLL mscs') sm hm' \/
+      [[ r = OK tt ]] * exists d tree' f' ilist' frees',
+        LOG.rep (FSXPLog fsxp) (SB.rep fsxp) (LOG.NoTxn (pushd d ds)) (MSLL mscs') sm hm' *
+        [[[ d ::: (Fm * DirTreeRep.rep fsxp Ftop tree' ilist' frees' mscs' sm)]]] *
+        [[ tree' = update_subtree pathname (TreeFile inum f') tree ]] *
+        [[ f' = mk_dirfile (setlen (DFData f) sz ($0, nil)) (DFAttr f) ]]
+    REC:vm',hm' RET:r exists mscs fsxp,
+      (exists d sm' n, LOG.rep (FSXPLog fsxp) (SB.rep fsxp) (LOG.NoTxn (d, nil)) (MSLL mscs) sm' hm' *
+         [[ n <= length (snd ds) ]] *
+         [[[ d ::: crash_xform (diskIs (list2nmem (nthd n ds))) ]]]) \/
+      (exists d dnew n sm' ds' tree' f' ilist' frees',
+         LOG.rep (FSXPLog fsxp) (SB.rep fsxp) (LOG.NoTxn (d, nil)) (MSLL mscs) sm' hm' *
+         [[ n <= length (snd ds') ]] *
+         [[[ d ::: crash_xform (diskIs (list2nmem (nthd n ds'))) ]]] *
+         [[ ds' = pushd dnew ds ]] *
+         [[[ dnew ::: (Fm * DirTreeRep.rep fsxp Ftop tree' ilist' frees' mscs sm')]]] *
+         [[ tree' = update_subtree pathname (TreeFile inum f') tree ]] *
+         [[ f' = mk_dirfile (setlen (DFData f) sz ($0, nil)) (DFAttr f) ]])
+     >>} file_truncate fsxp inum sz mscs >> recover cachesize.
+  Proof.
+    unfold forall_helper; intros.
+    (* workaround an evar tracking bug by destructing before instantiating;
+     otherwise proof goes through but at Qed time the variable d, produced from
+     v, cannot be found. *)
+    destruct v.
+    eexists; intros.
+    recover_ro_ok.
+    cancel.
+    eauto.
+    safestep.  (* crucial to use safe version *)
+    or_l.
+    cancel. cancel.
+
+    apply instantiate_crash.
+    cancel.
+    cancel.
+
+    cancel.
+
+    eassign_idempred.
+    cancel.
+
+    simpl.
+    repeat xform_dist.
+    repeat xform_deex_l.
+    xform_dist.
+    rewrite crash_xform_lift_empty.
+    norml. unfold stars; simpl. rewrite H9.
+
+    denote! (crash_xform F_ =p=> F_) as HFidem. rewrite HFidem.
+    xform_dist. norml; unfold stars; simpl.
+    - rewrite LOG.idempred_idem.
+      norml; unfold stars; simpl.
+      rewrite SB.crash_xform_rep.
+      cancel.
+
+      prestep. norm. cancel.
+      or_l. norm. cancel. intuition eassumption.
+
+      intuition eauto.
+      apply sep_star_lift_l; intros; apply pimpl_refl.
+
+      apply sep_star_lift_l; intros.
+      norm; unfold stars; simpl.
+      cancel.
+
+      split. constructor.
+      split. constructor.
+      denote! (crash_xform realcrash =p=> crash_xform _) as Hcr.
+      rewrite Hcr; clear Hcr.
+
+      rewrite <- LOG.before_crash_idempred. xform_dist. cancel.
+
+    - xform_norm.
+      rewrite LOG.idempred_idem.
+      norml; unfold stars; simpl.
+      rewrite SB.crash_xform_rep.
+      cancel.
+
+      prestep. norm. cancel.
+      or_r. norm. cancel. intuition idtac. 2: eauto. eauto.
+(*
+      pred_apply; cancel.
+
+      intuition eauto.
+      apply sep_star_lift_l; intros; apply pimpl_refl.
+
+      apply sep_star_lift_l; intros.
+      norm; unfold stars; simpl.
+      cancel.
+
+      split. constructor.
+      split. constructor.
+      denote! (crash_xform realcrash =p=> crash_xform _) as Hcr.
+      rewrite Hcr; clear Hcr.
+
+      xform_dist. or_r.
+      repeat ( progress xform_norm; cancel ).
+      rewrite <- LOG.before_crash_idempred.
+      unfold pushd; simpl; cancel.
+
+      pred_apply; cancel.
+*)
+  Grab Existential Variables.
+    all: try exact emp.
+  Qed.
+
+  Theorem update_fblock_d_recover_ok : forall fsxp inum off v mscs,
+    {<< ds sm Fm Ftop tree pathname f Fd vs frees ilist,
+    PRE:hm
+      LOG.rep (FSXPLog fsxp) (SB.rep fsxp) (LOG.NoTxn ds) (MSLL mscs) sm hm *
+      [[[ ds!! ::: (Fm * DirTreeRep.rep fsxp Ftop tree ilist frees mscs sm)]]] *
+      [[ find_subtree pathname tree = Some (TreeFile inum f) ]] *
+      [[[ (DFData f) ::: (Fd * off |-> vs) ]]]
+    POST:hm' RET:^(mscs')
+      exists tree' f' ds' sm',
+       LOG.rep (FSXPLog fsxp) (SB.rep fsxp) (LOG.NoTxn ds') (MSLL mscs') sm' hm' *
+       [[[ ds'!! ::: (Fm  * DirTreeRep.rep fsxp Ftop tree' ilist frees mscs' sm') ]]] *
+       [[ tree' = update_subtree pathname (TreeFile inum f') tree ]] *
+       [[[ (DFData f') ::: (Fd * off |-> (v, vsmerge vs)) ]]] *
+       [[ DFAttr f' = DFAttr f ]]
+    REC:vm',hm' RET:r exists mscs fsxp,
+      exists d sm', LOG.rep (FSXPLog fsxp) (SB.rep fsxp) (LOG.NoTxn (d, nil)) (MSLL mscs) sm' hm' *
+      ((exists n, 
+        [[[ d ::: crash_xform (diskIs (list2nmem (nthd n ds))) ]]] ) \/
+       (exists tree' f' v' ilist' frees',
+        [[[ d ::: (crash_xform Fm * DirTreeRep.rep fsxp Ftop tree' ilist' frees' mscs sm)]]] *
+        [[ tree' = update_subtree pathname (TreeFile inum f') tree ]] *
+        [[[ (DFData f') ::: (crash_xform Fd * off |=> v') ]]] *
+        [[ DFAttr f' = DFAttr f ]] *
+        [[ In v' (v :: vsmerge vs) ]]))
+   >>} update_fblock_d fsxp inum off v mscs >> recover cachesize.
+  Proof.
+    recover_ro_ok. 
+(*
+    cancel.
+    instantiate (pathname := v4); eauto.
+    eauto.
+    step.
+    apply pimpl_refl.
+*)
+    (* follows one of the earlier recover proofs but isn't used by atomiccp. *)
+  Admitted.
+
+  Hint Extern 0 (okToUnify (DirTreePred.tree_pred _ _) (DirTreePred.tree_pred _ _)) => constructor : okToUnify.
+
+  Theorem file_sync_recover_ok : forall fsxp inum mscs,
+    {<< ds sm Fm Ftop tree pathname f frees ilist,
+    PRE:hm
+      LOG.rep (FSXPLog fsxp) (SB.rep fsxp) (LOG.NoTxn ds) (MSLL mscs) sm hm *
+      [[[ ds!! ::: (Fm * DirTreeRep.rep fsxp Ftop tree ilist frees mscs sm)]]] *
+      [[ find_subtree pathname tree = Some (TreeFile inum f) ]]
+    POST:hm' RET:^(mscs')
+      exists ds' sm' tree' al,
+        LOG.rep (FSXPLog fsxp) (SB.rep fsxp) (LOG.NoTxn ds') (MSLL mscs') sm hm' *
+        [[ ds' = dssync_vecs ds al ]] *
+        [[[ ds'!! ::: (Fm * DirTreeRep.rep fsxp Ftop tree' ilist frees mscs' sm')]]] *
+        [[ tree' = update_subtree pathname (TreeFile inum (synced_dirfile f)) tree ]]
+    REC:vm',hm' RET:r exists mscs fsxp,
+      exists d,
+       LOG.rep (FSXPLog fsxp) (SB.rep fsxp) (LOG.NoTxn (d, nil)) (MSLL mscs) sm hm' *
+       ((exists n,  [[[ d ::: crash_xform (diskIs (list2nmem (nthd n ds))) ]]]) \/
+         exists flist' F' IFs,
+         [[[ d ::: (F' * BFILE.rep (FSXPBlockAlloc fsxp) IFs (FSXPInode fsxp) flist' ilist frees
+                                   (BFILE.MSAllocC mscs) (BFILE.MSCache mscs) (BFILE.MSICache mscs) (BFILE.MSDBlocks mscs)) ]]] *
+         [[[ flist' ::: (arrayN_ex (@ptsto _ addr_eq_dec _) flist' inum *
+                         exists c, inum |-> BFILE.synced_file (dirfile_to_bfile f c)) ]]]
+       )
+   >>} file_sync fsxp inum mscs >> recover cachesize.
+  Proof.
+    intros.
+    recover_ro_ok.
+    cancel. eauto.
+    step.
+
+    (* build a new idemcrash predicate that carries the XCRASH facts *)
+    instantiate (1 :=  (fun hm => (exists p, p * [[ crash_xform p =p=> crash_xform
+         (LOG.idempred (FSXPLog fsxp) (SB.rep fsxp) v hm
+      \/ (exists d tree',
+           LOG.idempred (FSXPLog fsxp) (SB.rep fsxp) (d, []) sm hm *
+           [[[ d ::: v0 ✶ DirTreeRep.rep fsxp v1 tree' v6 v5 mscs ]]] *
+           [[ tree' = update_subtree v3 (TreeFile inum (synced_dirfile v4)) v2 ]])) ]]))%pred).
+    apply pimpl_refl.
+    cancel. xform_dist. cancel.
+    simpl.
+    repeat xform_dist.
+    repeat xform_deex_l.
+    xform_dist.
+    rewrite crash_xform_lift_empty.
+    norml. unfold stars; simpl. rewrite H9.
+    xform_dist. xform_deex_l.
+
+    - rewrite LOG.idempred_idem; xform_deex_l;
+      rewrite SB.crash_xform_rep.
+      cancel.
+
+      prestep. norm. cancel.
+      recover_ro_ok.
+      cancel.
+      instantiate (mscs0 := ms).
+      cancel.
+      or_l; cancel.
+      setoid_rewrite <- surjective_pairing.
+      cancel.
+
+      intuition.
+      cancel.
+
+      simpl_idempred_r.
+      or_l; cancel.
+      rewrite <- LOG.before_crash_idempred.
+      auto.
+
+    - repeat xform_deex_l.
+      repeat xform_dist.
+      rewrite LOG.idempred_idem; xform_deex_l;
+      rewrite SB.crash_xform_rep.
+      cancel.
+
+      step.
+      denote crash_xform as Hx.
+      replace n with 0 in Hx by omega; rewrite nthd_0 in Hx; simpl in Hx.
+      denote! (_ (list2nmem x1)) as Hy.
+      apply (crash_xform_diskIs_pred _ Hy) in Hx.
+      apply crash_xform_sep_star_dist in Hx.
+
+      (* unfold DirTreeRep.rep in Hx to extract the file list *)
+      unfold DirTreeRep.rep in Hx; apply sep_star_comm in Hx.
+      repeat (rewrite crash_xform_exists_comm in Hx;
+        apply pimpl_exists_r_star_r in Hx;
+        destruct Hx as [ ? Hx ]).
+      repeat rewrite crash_xform_sep_star_dist in Hx.
+      repeat rewrite crash_xform_lift_empty in Hx.
+      rewrite BFILE.xform_rep, IAlloc.xform_rep in Hx.
+      destruct_lift Hx.
+      recover_ro_ok. cancel.
+      instantiate (mscs0 := BFILE.mk_memstate _ (MSLL ms) _ _ _ _). cancel.
+      or_r; cancel.
+
+      eapply pimpl_apply; [| eapply DirTreePred.flist_crash_synced_file; eauto].
+      cancel.
+      pred_apply; cancel.
+
+      simpl_idempred_r.
+      or_r; cancel.
+      do 3 (xform_norm; cancel).
+      rewrite <- LOG.before_crash_idempred.
+      eauto.
+      auto.
+
+    Unshelve.
+      all: eauto.
+      all: try solve [do 5 econstructor].
+  Qed.
+
+(*
+  Theorem lookup_recover_ok : forall fsxp dnum fnlist mscs,
+    {<< ds Fm Ftop tree ilist frees,
+    PRE:hm
+     LOG.rep (FSXPLog fsxp) (SB.rep fsxp) (LOG.NoTxn ds) (MSLL mscs) sm hm *
+      [[[ ds!! ::: (Fm * DirTreeRep.rep fsxp Ftop tree ilist frees) ]]] *
+      [[ DIRTREE.dirtree_inum tree = dnum]] *
+      [[ DIRTREE.dirtree_isdir tree = true ]]
+    POST:hm' RET:^(mscs',r)
+      LOG.rep (FSXPLog fsxp) (SB.rep fsxp) (LOG.NoTxn ds) (MSLL mscs') sm hm' *
+      [[ r = DIRTREE.find_name fnlist tree ]]
+    REC:hm' RET:^(mscs, fsxp)
+      exists d, LOG.rep (FSXPLog fsxp) (SB.rep fsxp) (LOG.NoTxn (d, nil)) mscs hm' *
+       [[[ d ::: crash_xform (diskIs (list2nmem (fst ds))) ]]]
+    >>} lookup fsxp dnum fnlist mscs >> recover cachesize.
+  Proof.
+    recover_ro_ok.
+    cancel.
+    eauto.
+    step.
+    instantiate (1 := (LOG.idempred (FSXPLog fsxp) (SB.rep fsxp) v \/
+      (exists cs : cachestate, LOG.after_crash (FSXPLog fsxp) (SB.rep fsxp) (fst v, []) cs))%pred).
+    cancel; cancel.
+    cancel.
+    or_l.
+    cancel.
+    xform_norm.
+    recover_ro_ok.
+    rewrite LOG.crash_xform_intact.
+    xform_norm.
+    rewrite SB.crash_xform_rep.
+
+    cancel.
+    rewrite LOG.notxn_after_crash_diskIs. cancel.
+    rewrite nthd_0; eauto. omega.
+
+    safestep; subst.
+    eassign d0; eauto.
+    pred_apply; instantiate (1 := nil).
+    replace n with 0 in *.
+    rewrite nthd_0; simpl; auto.
+    simpl in *; omega.
+
+    cancel; cancel.
+    rewrite LOG.after_crash_idem.
+    xform_norm.
+    rewrite SB.crash_xform_rep.
+    recover_ro_ok.
+    cancel.
+
+    step.
+    cancel; cancel.
+  Qed.
+*)
+
+(*
+  Theorem create_recover_ok : forall fsxp dnum name mscs,
+    {<< ds pathname Fm Ftop tree tree_elem ilist frees,
+    PRE:hm
+      LOG.rep (FSXPLog fsxp) (SB.rep fsxp) (LOG.NoTxn ds) (MSLL mscs) sm hm *
+      [[[ ds!! ::: (Fm * DirTreeRep.rep fsxp Ftop tree ilist frees) ]]] *
+      [[ DIRTREE.find_subtree pathname tree = Some (DIRTREE.TreeDir dnum tree_elem) ]]
+    POST:hm' RET:^(mscs',r)
+       [[ r = None ]] *
+        LOG.rep (FSXPLog fsxp) (SB.rep fsxp) (LOG.NoTxn ds) (MSLL mscs') sm hm'
+      \/ exists inum,
+       [[ r = Some inum ]] * exists d tree' ilist' frees',
+       LOG.rep (FSXPLog fsxp) (SB.rep fsxp) (LOG.NoTxn (pushd d ds)) (MSLL mscs') sm hm' *
+       [[ tree' = DIRTREE.tree_graft dnum tree_elem pathname name 
+                           (TreeFile inum BFILE.bfile0) tree ]] *
+       [[[ d ::: (Fm * DirTreeRep.rep fsxp Ftop tree' ilist' frees') ]]]
+    REC:hm' RET:^(mscs,fsxp)
+      exists d,
+      LOG.rep (FSXPLog fsxp) (SB.rep fsxp) (LOG.NoTxn (d, nil)) mscs hm' *
+      [[[ d ::: crash_xform (diskIs (list2nmem (fst ds))) ]]]
+    >>} create fsxp dnum name mscs >> recover cachesize.
+  Proof.
+    recover_ro_ok.
+    cancel.
+    eauto.
+    safestep.
+    or_l.
+    cancel.
+    subst.
+    apply pimpl_refl.
+    or_r.
+    cancel.
+    subst.
+    apply pimpl_refl.
+
+    (* if CRASH is LOG.idempred, we must manually instantiate idemcrash to include
+       the after_crash case *)
+    eassign ( LOG.idempred (FSXPLog fsxp) (SB.rep fsxp) v \/
+      (exists cs : cachestate, LOG.after_crash (FSXPLog fsxp) (SB.rep fsxp) (fst v, []) cs))%pred.
+    cancel; cancel.
+    xform_norm; recover_ro_ok.
+
+    - rewrite LOG.crash_xform_intact.
+      xform_norm.
+      rewrite SB.crash_xform_rep.
+      rewrite LOG.notxn_after_crash_diskIs with (n := 0) (ds := (fst v, nil)); auto.
+      cancel.
+      safestep.
+      cancel.
+      pred_apply; subst.
+      replace n with 0 by omega.
+      rewrite nthd_0; eauto.
+      cancel; cancel.
+
+    - rewrite LOG.after_crash_idem.
+      xform_norm.
+      rewrite SB.crash_xform_rep.
+      cancel.
+      step.
+      cancel; cancel.
+  Qed.
+*)
+
+(*
+  Theorem rename_recover_ok : forall fsxp dnum srcpath srcname dstpath dstname mscs,
+    {<< ds Fm Ftop tree cwd tree_elem ilist frees,
+    PRE:hm
+      LOG.rep (FSXPLog fsxp) (SB.rep fsxp) (LOG.NoTxn ds) (MSLL mscs) sm hm *
+      [[[ ds!! ::: (Fm * DirTreeRep.rep fsxp Ftop tree ilist frees) ]]] *
+      [[ DIRTREE.find_subtree cwd tree = Some (DIRTREE.TreeDir dnum tree_elem) ]]
+    POST:hm' RET:^(mscs',ok)
+      [[ ok = false ]] * LOG.rep (FSXPLog fsxp) (SB.rep fsxp) (LOG.NoTxn ds) (MSLL mscs') sm hm' \/
+      [[ ok = true ]] * 
+        rename_rep ds mscs' Fm fsxp Ftop tree ilist frees cwd dnum srcpath srcname dstpath dstname hm'
+    REC:hm' RET:^(mscs,fsxp)
+      exists d,
+        LOG.rep (FSXPLog fsxp) (SB.rep fsxp) (LOG.NoTxn (d, nil)) mscs hm' *
+        [[[ d ::: crash_xform (diskIs (list2nmem (fst ds))) ]]]
+    >>} rename fsxp dnum srcpath srcname dstpath dstname mscs >> recover cachesize.
+  Proof.
+    recover_ro_ok.
+    cancel.
+    eauto.
+    safestep.
+    or_l.
+    cancel.
+    subst.
+    apply pimpl_refl.
+    or_r.
+    cancel.
+    subst.
+    apply pimpl_refl.
+
+    (* if CRASH is LOG.idempred, we must manually instantiate idemcrash to include
+       the after_crash case *)
+    eassign ( LOG.idempred (FSXPLog fsxp) (SB.rep fsxp) v \/
+      (exists cs : cachestate, LOG.after_crash (FSXPLog fsxp) (SB.rep fsxp) (fst v, []) cs))%pred.
+    cancel; cancel.
+    xform_norm; recover_ro_ok.
+
+    - rewrite LOG.crash_xform_intact.
+      xform_norm.
+      rewrite SB.crash_xform_rep.
+      rewrite LOG.notxn_after_crash_diskIs with (n := 0) (ds := (fst v, nil)); auto.
+      cancel.
+      safestep.
+      cancel.
+      pred_apply; subst.
+      replace n with 0 by omega.
+      rewrite nthd_0; eauto.
+      cancel; cancel.
+
+    - rewrite LOG.after_crash_idem.
+      xform_norm.
+      rewrite SB.crash_xform_rep.
+      cancel.
+      step.
+      cancel; cancel.
+  Qed.
+*)
+
+End AFS_RECOVER.
