src/DiskSecVictim.v
@@ -192,3 +192,107 @@ Set Implicit Arguments.
     - eapply exec_same_except_failed in H; eauto; cleanup.
       right; right; repeat eexists; eauto.
   Qed.
+
+  
+
+   Lemma exec_same_except_rfinished:
+  forall T T' (p1: prog T) (p2: prog T') pr d d' bm bm' hm t d1 bm1 hm1 r1 tr,
+    exec_recover pr d bm hm p1 p2 (RFinished T' d1 bm1 hm1 r1) tr ->
+    same_except t d d' ->
+    blockmem_same_except t bm bm' ->
+    only_public_operations tr ->
+    t <> Public ->
+    exists d2 bm2,
+      exec_recover pr d' bm' hm p1 p2 (RFinished T' d2 bm2 hm1 r1) tr /\
+      same_except t d1 d2 /\
+      blockmem_same_except t bm1 bm2.
+  Proof.
+    intros.
+    inversion H; subst.
+    eapply exec_same_except_finished in H15; eauto; cleanup.
+    do 2 eexists; intuition eauto.
+    econstructor; eauto.
+  Qed.
+
+  Lemma exec_same_except_rfailed:
+  forall T T' (p1: prog T) (p2: prog T') pr d d' bm bm' hm t d1 bm1 hm1 tr,
+    exec_recover pr d bm hm p1 p2 (RFailed T T' d1 bm1 hm1) tr ->
+    same_except t d d' ->
+    blockmem_same_except t bm bm' ->
+    only_public_operations tr ->
+    t <> Public ->
+    exists d2 bm2,
+      exec_recover pr d' bm' hm p1 p2 (RFailed T T' d2 bm2 hm1) tr /\
+      same_except t d1 d2 /\
+      blockmem_same_except t bm1 bm2.
+  Proof.
+    intros.
+    inversion H; subst.
+    eapply exec_same_except_failed in H14; eauto; cleanup.
+    do 2 eexists; intuition eauto.
+    econstructor; eauto.
+  Qed.
+
+
+    Lemma exec_same_except_recover:
+  forall T T' (p1: prog T) (p2: prog T') pr d bm hm out tr,
+    exec_recover pr d bm hm p1 p2 out tr ->
+  forall t d',
+    same_except t d d' ->
+  forall bm',  
+    blockmem_same_except t bm bm' ->
+    only_public_operations tr ->
+    t <> Public ->
+    
+    (exists d1 bm1 hm1 r1 d2 bm2,
+      out = RFinished T' d1 bm1 hm1 r1 /\
+      exec_recover pr d' bm' hm p1 p2 (RFinished T' d2 bm2 hm1 r1) tr /\
+      same_except t d1 d2 /\
+      blockmem_same_except t bm1 bm2) \/
+    
+    (exists d1 bm1 hm1 d2 bm2,
+      out = RFailed T T' d1 bm1 hm1 /\
+      exec_recover pr d' bm' hm p1 p2 (RFailed T T' d2 bm2 hm1) tr /\
+      same_except t d1 d2 /\
+      blockmem_same_except t bm1 bm2) \/
+    
+    (exists d1 bm1 hm1 r1 d2 bm2,
+      out = RRecovered T d1 bm1 hm1 r1 /\
+      exec_recover pr d' bm' hm p1 p2 (RRecovered T d2 bm2 hm1 r1) tr /\
+      same_except t d1 d2 /\
+      blockmem_same_except t bm1 bm2).
+  Proof.
+    induction 1; intros.
+    { (** p1 finished **)
+      left; eapply exec_same_except_finished in H; eauto; cleanup.
+      do 6 eexists; intuition eauto.
+      econstructor; eauto.
+    }
+    { (** p1 failed **)
+      right; left; eapply exec_same_except_failed in H; eauto; cleanup.
+      do 5 eexists; intuition eauto.
+      econstructor; eauto.
+    }
+    { (** p1 crashed then p2 finished **)
+      clear IHexec_recover.
+      inversion H1; subst; clear H1.
+      apply only_public_operations_app in H4; cleanup.
+      eapply exec_same_except_crashed in H; eauto; cleanup.
+      eapply possible_crash_same_except in H6 as Hx; eauto; cleanup.
+      eapply exec_same_except_finished in H17 as Hp2; eauto; cleanup.
+      right; right; do 6 eexists; repeat split; eauto.
+      repeat (econstructor; eauto).
+      apply blockmem_same_except_refl.
+    }
+    { (** p1 crashed then p2 crashed **)
+      apply only_public_operations_app in H4; cleanup.
+      eapply exec_same_except_crashed in H; eauto; cleanup.
+      eapply possible_crash_same_except in H7 as Hx; eauto; cleanup.
+      specialize IHexec_recover with (1:=H10)(2:=@blockmem_same_except_refl t empty_mem)
+                                     (3:=H4)(4:=H5).
+      repeat split_ors; cleanup; try congruence.
+      inversion H11; subst; clear H11.
+      right; right; do 6 eexists; repeat split; eauto.
+      eapply XRCrashedRecovered; eauto.
+    }
+  Qed.
