src/Idempotent.v
@@ -1,0 +1,333 @@
+Require Import Hoare.
+Require Import Prog ProgMonad.
+Require Import Pred PredCrash.
+Require Import SepAuto.
+Require Import AsyncDisk.
+Require Import Hashmap.
+
+
+Lemma hashmap_subset_some_list_trans : forall hm hm' hm'',
+    (exists l, hashmap_subset l hm hm') ->
+    (exists l, hashmap_subset l hm' hm'') ->
+    exists l, hashmap_subset l hm hm''.
+Proof.
+  intros; solve_hashmap_subset.
+Qed.
+
+Lemma finished_val_eq : forall T m vm hm (v:T),
+    exists v', Finished m vm hm v = Finished m vm hm v'.
+Proof. eauto. Qed.
+
+Hint Resolve finished_val_eq.
+
+Lemma exec_crashed_hashmap_subset' : forall T (p: prog T) m m' bm bm' hm hm' out tr pr,
+  exec pr m bm hm p out tr
+  -> (out = Crashed m' bm' hm' \/ exists v, out = Finished m' bm' hm' v)
+  -> exists l, hashmap_subset l hm hm'.
+Proof.
+  intros.
+  generalize dependent bm'.
+  generalize dependent hm'.
+  generalize dependent m'.
+  
+  
+    induction H; subst; try solve [ intuition; repeat deex; try congruence;
+    try match goal with
+        | [ H: @eq (result) _ _ |- _ ] =>
+          inversion H; subst
+        end;
+    eauto; solve_hashmap_subset].
+
+    intros.
+    split_ors.    
+    eauto 10 using hashmap_subset_some_list_trans.
+    eauto 7 using hashmap_subset_some_list_trans.
+Qed.
+
+Lemma exec_crashed_blockmem_subset' : forall T (p: prog T) m m' bm bm' hm hm' out tr pr,
+  exec pr m bm hm p out tr
+  -> (out = Crashed m' bm' hm' \/ exists v, out = Finished m' bm' hm' v)
+  -> bm c= bm'.
+Proof.
+  intros.
+  generalize dependent bm'.
+  generalize dependent hm'.
+  generalize dependent m'.
+  
+  
+    induction H; subst; try solve [ intuition; repeat deex; try congruence;
+    try match goal with
+        | [ H: @eq (result) _ _ |- _ ] =>
+          inversion H; subst
+        end;
+    eauto; solve_hashmap_subset].
+
+    intros.
+    split_ors.    
+    eauto 10 using hashmap_subset_some_list_trans.
+    eauto 7 using hashmap_subset_some_list_trans.
+Qed.
+
+Lemma exec_crashed_hashmap_subset : forall T (p: prog T) pr tr m m' bm hm bm' hm' out,
+  exec pr m bm hm p out tr
+  -> out = Crashed  m' bm' hm'
+  -> exists l, hashmap_subset l hm hm'.
+Proof.
+  intros.
+  eapply exec_crashed_hashmap_subset'; eauto.
+Qed.
+
+Lemma exec_crashed_blockmem_subset : forall T (p: prog T) pr tr m m' bm hm bm' hm' out,
+  exec pr m bm hm p out tr
+  -> out = Crashed  m' bm' hm'
+  -> bm c= bm'.
+Proof.
+  intros.
+  eapply exec_crashed_blockmem_subset'; eauto.
+Qed.
+
+(*
+Ltac solve_hashmap_subset' :=
+  match goal with
+  | [ H: exec _ _ _ _ (Crashed _ _ _), Hpre: forall (_ : hashmap), _ =p=> ?pre _ _ _
+      |- forall (_ : hashmap), _ =p=> ?pre _ _ _ ]
+    => eapply exec_crashed_hashmap_subset in H as H'; eauto;
+        intros;
+        eapply pimpl_trans; try apply Hpre;
+        autorewrite with crash_xform; cancel
+  | [ |- context[hashmap_subset] ]
+        => pred_apply; cancel
+  end; try solve [
+    repeat match goal with
+    | [ H: forall (_ : hashmap), _ =p=> _ |- _ ] => clear H
+    end; solve_hashmap_subset
+  ].
+ *)
+
+Lemma corr3_from_corr2_failed:
+  forall (TF TR: Type) pr tr m mr bmr hmr (p: prog TF) (r: prog TR) out
+         (crash: block_mem -> hashmap -> pred) ppre rpre crashdone_p crashdone_r,
+  exec_recover pr mr bmr hmr p r out tr
+  -> TF = TR
+  -> possible_crash m mr
+  -> crash bmr hmr m
+  -> (forall bm' hm', crash_xform (crash bm' hm'
+     * [[ exists l, hashmap_subset l hmr hm' ]] *
+     [[ bmr c= bm' ]])
+      =p=> ppre crashdone_p crash bm' hm')
+  -> (forall bm' hm', crash_xform (crash bm' hm'
+      * [[ exists l, hashmap_subset l hmr hm' ]] *
+     [[ bmr c= bm' ]])
+      =p=> rpre crashdone_r crash bm' hm')
+  -> {{ pr | ppre }} p
+  -> {{ pr | rpre }} r
+  -> forall mx bmx hmx, out <> RFailed TF TR mx bmx hmx.
+Proof.
+  intros.
+  generalize dependent m.
+  induction H; intros; try congruence.
+  - edestruct H5; eauto.
+    eapply H3. eapply crash_xform_apply; eauto.
+    pred_apply; cancel.
+    solve_hashmap_subset.
+    repeat (destruct H7; try congruence).
+Qed.
+
+Lemma corr3_from_corr2_finished:
+  forall (TF TR: Type) pr tr m mr bmr hmr (p: prog TF) (r: prog TR) out
+    (crash: block_mem -> hashmap -> pred) ppre rpre crashdone_p crashdone_r m' bm' hm' v,
+  exec_recover pr mr bmr hmr p r out tr
+  -> TF = TR
+  -> possible_crash m mr
+  -> crash bmr hmr m
+  -> (forall bm' hm', crash_xform (crash bm' hm'
+     * [[ exists l, hashmap_subset l hmr hm' ]] *
+     [[ bmr c= bm' ]])
+      =p=> ppre crashdone_p crash bm' hm')
+  -> (forall bm' hm', crash_xform (crash bm' hm'
+      * [[ exists l, hashmap_subset l hmr hm' ]] *
+     [[ bmr c= bm' ]])
+      =p=> rpre crashdone_r crash bm' hm')
+  -> {{ pr | ppre }} p
+  -> {{ pr | rpre }} r
+  -> out = RFinished TR m' bm' hm' v
+  -> crashdone_p m' bm' hm' v /\ only_public_operations tr.
+Proof.
+  intros.
+  induction H; try congruence.
+  edestruct H5; eauto.
+  - eapply H3. eapply crash_xform_apply; eauto.
+    pred_apply; cancel.
+    solve_hashmap_subset.
+  - split_ors; cleanup; try congruence; split; eauto; congruence.
+Qed.
+
+Lemma corr3_from_corr2_recovered:
+  forall (TF TR: Type) mr bmr hmr (p: prog TF) (r: prog TR) out
+         (crash: block_mem -> hashmap -> pred) ppre rpre crashdone_p crashdone_r m' bm' hm' v pr tr,
+  exec_recover pr mr bmr hmr p r out tr
+  -> out = RRecovered TF m' bm' hm' v  
+  -> TF = TR
+  -> forall m,
+    possible_crash m mr
+  -> crash bmr hmr m
+  -> (forall bm' hm', crash_xform (crash bm' hm'
+     * [[ exists l, hashmap_subset l hmr hm' ]] *
+     [[ bmr c= bm' ]])
+      =p=> ppre crashdone_p crash bm' hm')
+  -> (forall bm' hm', crash_xform (crash bm' hm'
+      * [[ exists l, hashmap_subset l hmr hm' ]])
+      =p=> rpre crashdone_r crash bm' hm')
+  -> (forall bm hm, crash bm hm =p=> crash Mem.empty_mem hm)
+  -> {{ pr | ppre }} p
+  -> {{ pr | rpre }} r
+  -> crashdone_r m' bm' hm' v /\ only_public_operations tr.
+Proof.
+  induction 1; intros; try congruence.
+  - inversion H2; subst; clear H2.
+    edestruct H9; eauto.
+    eapply H6; eapply crash_xform_apply; eauto.
+    pred_apply; cancel.
+    solve_hashmap_subset.
+    split_ors; cleanup; try congruence.
+    inversion H1; subst.
+    edestruct H10; eauto.
+    
+    eapply H7; eapply crash_xform_apply; eauto.
+    pred_apply; cancel.
+    eauto.
+    eapply exec_crashed_hashmap_subset; eauto.
+    split_ors; cleanup; try congruence.
+    split; eauto.
+    apply only_public_operations_app_merge; eauto.
+    
+  - inversion H2; subst; clear H2.
+    edestruct H9; eauto.
+    eapply H6; eapply crash_xform_apply; eauto.
+    pred_apply; cancel.
+    solve_hashmap_subset.
+    split_ors; cleanup; try congruence.
+    edestruct IHexec_recover; eauto.
+    eapply H8; eauto.
+
+    intros.
+    repeat rewrite crash_xform_sep_star_dist.
+    xcrash.
+    rewrite <- H7; cancel.
+    rewrite crash_xform_sep_star_dist.
+    cancel.
+    rewrite crash_xform_lift_empty; cancel.
+    eapply hashmap_subset_some_list_trans; eauto.
+    eapply exec_crashed_hashmap_subset; eauto.
+
+    intros.
+    repeat rewrite crash_xform_sep_star_dist.
+    xcrash.
+    rewrite <- H7; cancel.
+    rewrite crash_xform_sep_star_dist.
+    cancel.
+    rewrite crash_xform_lift_empty; cancel.
+    eapply hashmap_subset_some_list_trans; eauto.
+    eapply exec_crashed_hashmap_subset; eauto.
+    split; eauto.
+    apply only_public_operations_app_merge; eauto.
+Qed.
+
+Theorem corr3_from_corr2:
+  forall TF TR (p: prog TF) (r: prog TR) pr ppre rpre,
+    {{ pr | ppre }} p
+  -> {{ pr | rpre }} r                 
+  -> {{ pr | fun bm hm done crashdone => exists crash,
+        ppre done crash bm hm
+        * [[ forall bm hm, crash bm hm =p=> crash Mem.empty_mem hm ]]
+        * [[ forall bm' hm',
+          crash_xform (crash bm' hm'
+          * [[ exists l, hashmap_subset l hm hm' ]])
+          =p=> rpre crashdone crash bm' hm' ]] }} p >> r.
+Proof.
+  unfold corr3; intros.
+  destruct H1 as [crash H1].
+  destruct_lift H1.
+  inversion H2; subst.
+  - edestruct H; eauto.
+    split; eauto.
+    split_ors; cleanup; try congruence.
+    left; repeat eexists; eauto.
+  - exfalso.
+    edestruct H; eauto; repeat deex; try congruence.
+    split_ors; cleanup; try congruence.
+  - edestruct H; eauto; repeat deex; try congruence.
+    split_ors; cleanup; try congruence.
+    clear H H1 H2 ppre.    
+    inversion H7; subst.
+    edestruct H0; eauto.
+    eapply H5.
+    eapply crash_xform_apply; eauto.
+    pred_apply; cancel.
+    eauto.
+    eapply exec_crashed_hashmap_subset; eauto.
+    split_ors; cleanup; try congruence.
+    split.
+    right; repeat eexists; eauto.
+    apply only_public_operations_app_merge; eauto.
+    
+  - edestruct H; eauto; repeat deex; try congruence.
+    split_ors; cleanup; try congruence.
+    clear H H1 H2 ppre.
+    edestruct corr3_from_corr2_recovered.
+    apply H7.
+    all: eauto.
+    eapply H6; eauto.
+
+    intros.
+    repeat rewrite crash_xform_sep_star_dist.
+    xcrash.
+    rewrite <- H5; cancel.
+    rewrite crash_xform_sep_star_dist.
+    cancel.
+    rewrite crash_xform_lift_empty; cancel.
+    eapply hashmap_subset_some_list_trans; eauto.
+    eapply exec_crashed_hashmap_subset; eauto.
+
+    intros.
+    repeat rewrite crash_xform_sep_star_dist.
+    xcrash.
+    rewrite <- H5; cancel.
+    rewrite crash_xform_sep_star_dist.
+    cancel.
+    rewrite crash_xform_lift_empty; cancel.
+    eapply hashmap_subset_some_list_trans; eauto.
+    eapply exec_crashed_hashmap_subset; eauto.
+    split; eauto.
+    right; repeat eexists; eauto.
+    apply only_public_operations_app_merge; eauto.
+Qed.
+
+Theorem corr3_from_corr2_rx :
+  forall TF TR RF RR pr (p: prog TF) (r:  prog TR)
+         (rxp : TF -> prog RF) (rxr : TR -> prog RR)
+         ppre rpre,
+  {{ pr | ppre }} Bind p rxp
+  -> {{ pr | rpre }} Bind r rxr
+  -> {{ pr | fun bm hm done crashdone => exists crash,
+        ppre done crash bm hm
+        * [[ forall bm hm, crash bm hm =p=> crash Mem.empty_mem hm ]]        
+        * [[ forall bm' hm',
+          crash_xform (crash bm' hm'
+          * [[ exists l, hashmap_subset l hm hm' ]])
+          =p=> rpre crashdone crash bm' hm']] }} Bind p rxp >> Bind r rxr.
+Proof.
+  intros.
+  apply corr3_from_corr2; eauto.
+Qed.
+
+  Ltac recover_ro_ok := intros;
+    repeat match goal with
+      | [ |- forall_helper _ ] => unfold forall_helper; intros; eexists; intros
+      | [ |- corr3 _ ?pre' _ _ ] => eapply corr3_from_corr2_rx; eauto with prog
+      | [ |- corr3 _ _ _ _ ] => eapply pimpl_ok3; intros
+      | [ |- corr2 _ _ _ ] => step
+      | [ H: crash_xform ?x =p=> ?x |- context [ crash_xform ?x ] ] => rewrite H
+      | [ H: diskIs _ _ |- _ ] => unfold diskIs in *
+      | [ |- pimpl (crash_xform _) _ ] => progress autorewrite with crash_xform
+    end.
